

THE PRESCRIBED CROSS CURVATURE PROBLEM ON THREE-DIMENSIONAL UNIMODULAR LIE GROUPS

BENJAMIN KRUGER

ABSTRACT. Let G be a three-dimensional unimodular Lie group and let T be a left-invariant $(0, 2)$ -tensor field on G . We study the necessary and sufficient conditions for the existence of a left-invariant metric g that satisfies the equation $X(g) = T$ on three-dimensional unimodular Lie groups, where $X(g)$ is the cross curvature of g . We discuss uniqueness of solutions for the groups $E(2)$, $E(1, 1)$, H_3 and \mathbb{R}^3 .

1. INTRODUCTION

The problem of prescribing curvature on a given manifold is a fundamental topic in Riemannian geometry. A particularly well-studied instance of this is the problem of prescribing Ricci curvature. Let M be a Riemannian manifold, and let T be a given $(0, 2)$ -tensor field. One is interested in the existence and uniqueness of a Riemannian metric g such that

$$\text{Ric}(g) = T. \quad (1.1)$$

Hamilton proved existence in the case where $M = \text{SU}(2)$ [Ham84]. Buttsworth later extended the result to \mathbb{S}^2 , $E(2)$, $E(1, 1)$, H_3 and \mathbb{R}^3 . Motivated by a restriction on the solvability of (1.1) on \mathbb{S}^2 [Ham84], [DeT16], and the scale invariance of the Ricci curvature, work on the prescribed Ricci curvature problem often considers (1.1) with a scalar multiple of T . In this paper, we study the analogue of this problem for the cross curvature tensor.

The cross curvature, introduced by Chow and Hamilton [CH04] in the context of uniformising three-manifolds, is a $(0, 2)$ -tensor field $X(g)$. Let M be a Riemannian manifold. The prescribed cross curvature problem asks for a given $(0, 2)$ -tensor field T , does there exist a Riemannian metric g such that,

$$X(g) = T. \quad (1.2)$$

Some existence and uniqueness results have been obtained when $M = \mathbb{S}^3$ [BP21], [Gki08]. We consider the particular problem of prescribing cross curvature of left-invariant metrics on three-dimensional unimodular Lie groups. Note that the cross curvature is not scaling invariant and hence we drop the scaling factor in (1.2).

Definition 1.1 (Einstein Tensor Field). Let (M, g) be a three-dimensional Riemannian manifold. Define the $(0, 2)$ -tensor field

$$\text{Ein}(g) := \text{Ric}(g) - g \frac{S}{2},$$

where S is the scalar curvature of M .

We find it useful to define the $(1, 1)$ -tensor

$$\mathcal{E}(g) = \left(\text{Ric}(g) - g \frac{S}{2} \right)^\#.$$

Definition 1.2 (Cross Curvature). The cross curvature tensor is

$$X(g)(\cdot, \cdot) := \det(\mathcal{E}) g(\mathcal{E}^{-1}\cdot, \cdot). \quad (1.3)$$

Gkigkitzis defines an analogous problem to (1.2) for the cross transformation, a $(1, 2)$ -tensor, and proves a result on the existence and uniqueness of left-invariant metrics on $SU(2)$ [Gki08]. Pulemotov and Buttsworth show that the two problems are equivalent [BP21].

Let \mathbf{G} be a three-dimensional unimodular Lie group with Lie algebra \mathfrak{g} . For any left-invariant metric g , there exists a basis $\{V_1, V_2, V_3\}$ of \mathfrak{g} that diagonalises the metric and gives us the Lie bracket relations:

$$[V_i, V_j] = \sum_{k=1}^3 \epsilon_{ijk} \lambda_k V_k \quad (1.4)$$

for some coefficients $\lambda_k \in \mathbb{R}$ [HL09]. The structure coefficients λ_k can be scaled and the basis of \mathfrak{g} can be oriented to uniquely describe each of the 6 unimodular three-dimensional Lie groups. In [But19], it was shown to be sufficient to consider values of λ_k in $\{-2, 0, 2\}$. We focus on the four groups in which at least one of the λ_k values is 0 and obtain the following result:

Theorem 1.3. Let T be a left-invariant $(0, 2)$ -tensor field on $\mathbf{E}(2)$, $\mathbf{E}(1, 1)$ or \mathbf{H}_3 . Then, there exists a left-invariant Riemannian metric g solving (1.2) if and only if:

- (i) T is diagonalisable in a basis $\{V_i\}_{i=1}^3$ in which (1.4) holds, and
- (ii) The diagonal elements $T(V_i, V_i) =: T_i$ have signature as in theorems 4.1, 4.2 and 4.3 $\mathbf{E}(2)$, $\mathbf{E}(1, 1)$ and \mathbf{H}_3 respectively.

In the same basis, if none of the diagonal elements T_i are zero, the solution g is unique.

2. THE CROSS CURVATURE TENSOR ON A UNIMODULAR LIE GROUP

In this section we compute the cross curvature tensor for a three-dimensional unimodular Lie group \mathbf{G} :

Lemma 2.1. Let (\mathbf{G}, g) be a three-dimensional unimodular Lie group with Lie algebra \mathfrak{g} . Let $\{V_i\}_{i=1}^3$ be a basis of \mathfrak{g} that diagonalises g . That is, $g = x_1 d\theta_1 + x_2 d\theta_2 + x_3 d\theta_3$ where $\{\theta_i\}_{i=1}^3$ is the basis of \mathfrak{g}^* . Then the cross curvature tensor is:

$$X(g)(V_i, V_j) = \delta_{ij} \frac{(\mathbf{x}_i \mathbf{x}_{i+2} - \mathbf{x}_{i+1} \mathbf{x}_{i+2} - \mathbf{x}_i \mathbf{x}_{i+1})(\mathbf{x}_i \mathbf{x}_{i+1} - \mathbf{x}_i \mathbf{x}_{i+2} - \mathbf{x}_{i+1} \mathbf{x}_{i+2})}{x_i x_{i+1}^2 x_{i+2}^2} \quad (2.1)$$

where $\mathbf{x}_i := \frac{\lambda_{i+2} x_{i+2} + \lambda_{i+1} x_{i+1} - \lambda_i x_i}{2}$ for $i = 1, 2, 3$.

Proof. Fix a basis $\{V_i\}_{i=1}^3$ in which (1.4) holds and g is diagonal. We first compute

$$\begin{aligned} g(\nabla_{V_i} V_{i+1}, V_{i+2}) &= \frac{1}{2} (g([V_i, V_{i+1}], V_{i+2}) - g([V_i, V_{i+2}], V_{i+1}) - g([V_{i+1}, V_{i+2}], V_i)), \\ &= \frac{1}{2} (g(\lambda_{i+2} V_{i+2}, V_{i+2}) - g(-\lambda_{i+1} V_{i+1}, V_{i+1}) - g(\lambda_i V_i, V_i)), \\ &= \frac{\lambda_{i+2} x_{i+2} + \lambda_{i+1} x_{i+1} - \lambda_i x_i}{2} \end{aligned}$$

by the Koszul formula:

$$g(\nabla_X Y, Z) = \frac{1}{2} (g([X, Y], Z) - g([X, Z], Y) - g([Y, Z], X)).$$

This gives us that

$$\nabla_{V_i} V_{i+1} = \frac{\lambda_{i+2} x_{i+2} + \lambda_{i+1} x_{i+1} - \lambda_i x_i}{2 x_{i+2}} V_{i+2}.$$

Since the Riemann curvature tensor is symmetric, we only need to compute $R(V_i, V_{i+1}, V_i, V_{i+1})$ for $i = 1, 2, 3$. We use the fact that $R(X, Y, X, Y) = g(R(X, Y)Y, X)$ to compute:

$$R(V_i, V_{i+1}, V_i, V_{i+1}) = \lambda_{i+2} \left(\mathbf{x}_{i+2} - \frac{\mathbf{x}_i \mathbf{x}_{i+1}}{\mathbf{x}_i + \mathbf{x}_{i+1}} \right)$$

and subsequently

$$\text{Ric}(V_i, V_j) = \delta_{ij} \frac{2 \mathbf{x}_{i+1} \mathbf{x}_{i+2}}{x_{i+1} x_{i+2}}.$$

The scalar curvature is then given by

$$\begin{aligned} S &= g^{ij} \text{Ric}(V_i, V_j), \\ &= \frac{1}{x_1} \frac{2 \mathbf{x}_2 \mathbf{x}_3}{x_2 x_3} + \frac{1}{x_2} \frac{2 \mathbf{x}_1 \mathbf{x}_3}{x_1 x_3} + \frac{1}{x_3} \frac{2 \mathbf{x}_1 \mathbf{x}_2}{x_1 x_2}, \\ &= \frac{2}{x_1 x_2 x_3} (\mathbf{x}_2 \mathbf{x}_3 + \mathbf{x}_1 \mathbf{x}_3 + \mathbf{x}_1 \mathbf{x}_2). \end{aligned}$$

We now have all the elements required to compute the $(1, 1)$ -tensor field $\mathcal{E}(g)$:

$$\mathcal{E}_j^i = g^{ik} \text{Ric}_{jk} - \frac{S}{2} \delta_j^i.$$

The off diagonal elements vanish and we are left with

$$\begin{aligned} \mathcal{E}_i^i &= \frac{1}{x_i} \frac{2 \mathbf{x}_{i+1} \mathbf{x}_{i+2}}{x_{i+1} x_{i+2}} - \frac{\frac{2}{x_1 x_2 x_3} (\mathbf{x}_{i+1} \mathbf{x}_{i+2} + \mathbf{x}_i \mathbf{x}_{i+2} + \mathbf{x}_i \mathbf{x}_{i+1})}{2}, \\ &= \frac{\mathbf{x}_{i+1} \mathbf{x}_{i+2} - \mathbf{x}_i \mathbf{x}_{i+2} - \mathbf{x}_i \mathbf{x}_{i+1}}{x_i^2 x_{i+1} x_{i+2}}. \end{aligned}$$

Using (1.3) we finally obtain

$$X(g)(V_i, V_j) = \delta_{ij} \frac{(\mathbf{x}_i \mathbf{x}_{i+2} - \mathbf{x}_{i+1} \mathbf{x}_{i+2} - \mathbf{x}_i \mathbf{x}_{i+1})(\mathbf{x}_i \mathbf{x}_{i+1} - \mathbf{x}_i \mathbf{x}_{i+2} - \mathbf{x}_{i+1} \mathbf{x}_{i+2})}{x_i x_{i+1}^2 x_{i+2}^2} \quad (2.2)$$

□

Given a basis in which T is diagonal with $T(V_i, V_j) = \delta_{ij}T_i$, we see that solving (1.2) is equivalent to solving the following system of equations:

$$\begin{cases} \frac{(\mathbf{x}_1\mathbf{x}_3 - \mathbf{x}_2\mathbf{x}_3 - \mathbf{x}_1\mathbf{x}_2)(\mathbf{x}_1\mathbf{x}_2 - \mathbf{x}_1\mathbf{x}_3 - \mathbf{x}_2\mathbf{x}_3)}{x_1^2x_2^2x_3^2} = T_1, \\ \frac{(\mathbf{x}_2\mathbf{x}_3 - \mathbf{x}_1\mathbf{x}_3 - \mathbf{x}_1\mathbf{x}_2)(\mathbf{x}_1\mathbf{x}_2 - \mathbf{x}_1\mathbf{x}_3 - \mathbf{x}_2\mathbf{x}_3)}{x_1^2x_2^2x_3^2} = T_2, \\ \frac{(\mathbf{x}_2\mathbf{x}_3 - \mathbf{x}_1\mathbf{x}_3 - \mathbf{x}_1\mathbf{x}_2)(\mathbf{x}_1\mathbf{x}_3 - \mathbf{x}_2\mathbf{x}_3 - \mathbf{x}_1\mathbf{x}_2)}{x_1^2x_2^2x_3} = T_3. \end{cases} \quad (2.3)$$

Recall here $\mathbf{x}_i = \frac{\lambda_{i+2}x_{i+2} + \lambda_{i+1}x_{i+1} - \lambda_i x_i}{2}$ for $i = 1, 2, 3$.

3. EXISTENCE AND UNIQUENESS

We present two lemmas analogous to Lemmas 3.1 and 3.2 in [But19].

Lemma 3.1. Let T be a left-invariant $(0, 2)$ -tensor field on a three-dimensional unimodular Lie group \mathbf{G} . There exists a left-invariant metric g solving (1.2) if and only if the following conditions hold:

- (i) There exists a basis $\{V_i\}_{i=1}^3$ of \mathfrak{g} satisfying (1.4) in which T is diagonal.
- (ii) There is a solution (x_1, x_2, x_3) of (2.3).

Lemma 3.2. Let T be a non-zero left-invariant $(0, 2)$ -tensor field on \mathbf{G} and let g be a left-invariant metric such that $X(g) = T$. The metric g is unique if the following hold:

- (i) Given a basis $\{V_i\}_{i=1}^3$ such that T is diagonal and (2.3) holds, then g is diagonal;
- (ii) The solution (x_1, x_2, x_3) of (2.3) is unique whenever T_1, T_2, T_3 are the diagonal components of T in a basis $\{V_i\}_{i=1}^3$ satisfying (1.4).

The following lemma from [But19] is utilised in conjunction with lemma 3.2 to give conditions on the uniqueness of solutions to (1.2).

Lemma 3.3. For $\mathbf{E}(2)$, $\mathbf{E}(1, 1)$, and \mathbf{H}_3 , let $U_i = \sum_{j=1}^3 a_{ji}V_j$ be the change of basis from $\{V_i\}_{i=1}^3$ that satisfies (1.4). If $\{U_i\}_{i=1}^3$ satisfies (1.4), the following constraints must be satisfied for a given value of λ_2 :

- (i) $\lambda_2 = 2$:

$$\begin{aligned} a_{31} &= a_{32} = 0, & a_{33} &= \pm 1, \\ a_{21} &= \mp a_{12}, & a_{11} &= \pm a_{22}. \end{aligned}$$

- (ii) $\lambda_2 = -2$:

$$\begin{aligned} a_{31} &= a_{32} = 0, & a_{33} &= \pm 1, \\ a_{21} &= \pm a_{12}, & a_{11} &= \pm a_{22}. \end{aligned}$$

- (iii) $\lambda_2 = 0$:

$$\begin{aligned} a_{11} &= a_{22}a_{33} - a_{32}a_{23}, \\ a_{21} &= a_{31} = 0. \end{aligned}$$

Condition (i) of lemma 3.2 amounts to showing that the change of basis maps diagonal matrices to diagonal matrices. We compute the change of basis for the matrix of T to be

$$A^T \begin{pmatrix} T_1 & 0 & 0 \\ 0 & T_2 & 0 \\ 0 & 0 & T_3 \end{pmatrix} A.$$

4

That is,

$$\begin{pmatrix} a_{11}^2 T_1 + a_{21}^2 T_2 + a_{31}^2 T_3 & a_{11}a_{12}T_1 + a_{21}a_{22}T_2 + a_{31}a_{32}T_3 & a_{11}a_{13}T_1 + a_{21}a_{23}T_2 + a_{31}a_{33}T_3 \\ a_{11}a_{12}T_1 + a_{21}a_{22}T_2 + a_{31}a_{32}T_3 & a_{12}^2 T_1 + a_{22}^2 T_2 + a_{32}^2 T_3 & a_{12}a_{13}T_1 + a_{22}a_{23}T_2 + a_{32}a_{33}T_3 \\ a_{11}a_{13}T_1 + a_{21}a_{23}T_2 + a_{31}a_{33}T_3 & a_{12}a_{13}T_1 + a_{22}a_{23}T_2 + a_{32}a_{33}T_3 & a_{13}^2 T_1 + a_{23}^2 T_2 + a_{33}^2 T_3 \end{pmatrix}$$

It is not hard to verify that if the above is diagonal and all $T_i \neq 0$, then

$$A^T \begin{pmatrix} x_1 & 0 & 0 \\ 0 & x_2 & 0 \\ 0 & 0 & x_3 \end{pmatrix} A$$

is also diagonal.

4. RESULTS FOR $E(2)$, $E(1,1)$ AND H_3

4.1. The Euclidean Group, $E(2)$.

Theorem 4.1. Let T be a left-invariant $(0,2)$ tensor field on $E(2)$. There exists a left-invariant metric g such that $X(g) = T$ if and only if T is diagonalisable in a basis $\{V_i\}_{i=1}^3$ satisfying (1.4) with $\lambda_1 = \lambda_2 = \lambda_3 = 2$ and exactly one of the following conditions is satisfied:

- (i) $T_1 = T_2 = T_3$,
- (ii) $T_1 > 0$ and $T_2, T_3 < 0$,
- (iii) $T_1, T_3 < 0$ and $T_2 > 0$.

In (i), there are infinitely many solutions. In (ii) and (iii), the solution g is unique.

Proof. Fix a basis $\{V_i\}_{i=1}^3$ of \mathfrak{g} in which T is diagonal and (1.4) holds. We compute the variables $\mathbf{x}_1 = x_2 - x_1$, $\mathbf{x}_2 = x_1 - x_2$, and $\mathbf{x}_3 = x_1 + x_2$. This simplifies (2.3) to

$$\begin{cases} T_1 = \frac{(x_1+3x_2)(x_1-x_2)^3}{x_1^2 x_2^2 x_3^2} \\ T_2 = \frac{-(3x_1+x_2)(x_1-x_2)^3}{x_1^2 x_2^2 x_3^2} \\ T_3 = \frac{-(x_2+3x_1)(3x_2+x_1)(x_1-x_2)^2}{x_1^2 x_2^2 x_3} \end{cases} \quad (4.1)$$

By the positive definiteness of g , we know that $T_3 \leq 0$ and T_2 is opposite in sign to T_1 . We proceed with three cases:

- (i) Assume $T_1 = 0$. As $x_1, x_2, x_3 > 0$ we know $x_1 = x_2$. This ensures $T_2 = T_3 = 0$. As there is no dependence on x_3 , there are infinite solutions g to (1.2).
- (ii) Assume $T_1 > 0$. From the first equation we have $x_3^2 = \frac{(x_1+3x_2)(x_1-x_2)^3}{x_1^2 x_2^2 T_1}$. Substituting this into the second equation we find, $0 = x_1^2 T_2 + 3x_1 x_2 (T_1 + T_2) + x_2^2 T_1$. This gives an expression for x_1 ,

$$x_1 = x_2 \frac{-3(T_1 + T_2) \pm (9T_1^2 + 14T_1 T_2 + 9T_2^2)^{\frac{1}{2}}}{2T_2}.$$

As $x_1 > 0$, we see $-3(T_1 + T_2) \pm (9T_1^2 + 14T_1 T_2 + 9T_2^2)^{\frac{1}{2}} < 0$. Since $-3(T_1 + T_2) < (9T_1^2 + 14T_1 T_2 + 9T_2^2)^{\frac{1}{2}}$, we may disregard the positive and solve uniquely for (x_1, x_2, x_3) .

- (iii) Assume $T_1 < 0$. This case is similar to the previous however as $T_2 > 0$, we disregard the negative of the square root in the expression for x_1 . Again we obtain a unique solution of (x_1, x_2, x_3) . This solves the existence of our metric.

In cases (ii) and (iii), we have that all $T_i \neq 0$ for $i = 1, 2, 3$. Thus, by the discussion in § 3, we apply lemma 3.2 to obtain uniqueness of the metric. \square

4.2. The Minkowski Group, $E(1, 1)$.

Theorem 4.2. Let T be a left-invariant $(0, 2)$ tensor field on $E(1, 1)$. There exists a left-invariant Riemannian metric g such that $X(g) = T$ if and only if T is diagonalisable in a basis $\{V_i\}_{i=1}^3$ satisfying (1.4) with $\lambda_1 = 2, \lambda_2 = -2, \lambda_3 = 0$ and one of the following conditions is satisfied:

- (i) $T_1 < 0, T_2 = T_3 = 0$,
- (ii) $T_1 = T_3 = 0, T_2 < 0$,
- (iii) $T_1 > 0, T_2, T_3 < 0$,
- (iv) $T_1 < 0, T_2, T_3 > 0$, and
- (v) $T_1, T_2, T_3 < 0$.

Here we denote $T_i = T(V_i, V_i)$. In (i) and (ii) there are infinitely many solutions g to (1.2). In (iii), (iv) and (v), the solution g is unique.

Proof. Fix a basis $\{V_i\}_{i=1}^3$ of \mathfrak{g} in which T is diagonal and (1.4) holds. We compute the variables $\mathbf{x}_1 = -(x_2 + x_1), \mathbf{x}_2 = x_2 + x_1, \mathbf{x}_3 = x_1 - x_2$. This simplifies (2.3) to

$$\begin{cases} T_1 = \frac{(x_1 - 3x_2)(x_1 + x_2)^3}{x_1 x_2^2 x_3^2} \\ T_2 = \frac{-(3x_1 - x_2)(x_1 + x_2)^3}{x_1^2 x_2 x_3^2} \\ T_3 = \frac{-(x_2 - 3x_1)(3x_2 - x_1)(x_1 + x_2)^2}{x_1^2 x_2^2 x_3} \end{cases} \quad (4.2)$$

It is clear that the five conditions on the signature T_i listed are exhaustive so we consider existence and uniqueness in each. For the last three conditions, it is useful to solve for x_3^2 and substitute the expression into the second equation, solving for x_1 . We find

$$x_3^2 = \frac{(x_1 - 3x_2)(x_1 + x_2)^3}{x_1 x_2^2 T_1},$$

and hence

$$x_1 = x_2 \frac{-3(T_1 - T_2) \pm (9T_1^2 - 14T_1 T_2 + 9T_2^2)^{\frac{1}{2}}}{2T_2}.$$

- (i) Given $T_2 = T_3 = 0$ we conclude that $3x_1 = x_2$ as $x_1, x_2, x_3 > 0$. This simplifies the first equation to $T_1 = \frac{-512x_1}{9x_3^2}$. This has infinitely many solutions.
- (ii) Given $T_1, T_3 = 0$, we find $T_2 = \frac{-512x_2}{9x_3^2}$. This has infinitely many solutions.

- (iii) Given $T_2, T_3 < 0$ and $T_1 > 0$, we require $x_1 \geq 3x_2$. This implies $3 \leq \frac{-3(T_1 - T_2) \pm (9T_1^2 - 14T_1 T_2 + 9T_2^2)^{\frac{1}{2}}}{2T_2}$ and so $3T_2 + 3T_1 \geq \pm (9T_1^2 - 14T_1 T_2 + 9T_2^2)^{\frac{1}{2}}$. This gives us two expressions, the first of which cannot hold since $T_2 < 0$. Thus we take the negative of the square root, giving us a single expression for x_1 in terms of x_2 . Substituting this into our expression for x_3 and finally into the third equation, we solve a unique expression for x_2 . We then recover expressions for x_1 and x_3 , giving us a unique solution.

- (iv) This case is similar to the previous, however we find $\frac{1}{3}x_2 \leq x_1 \leq 3x_2$ and so $\frac{1}{3} \leq \frac{-3(T_1-T_2) \pm (9T_1^2 - 14T_1T_2 + 9T_2^2)^{\frac{1}{2}}}{2T_2}$. Again this gives us two expressions,

$$\begin{aligned} \frac{49}{9}T_2^2 - 14T_1T_2 + 9T_1^2 &< 9T_2^2 - 14T_1T_2 + 9T_1^2 \\ \frac{49}{9}T_2^2 - 14T_1T_2 + 9T_1^2 &> 9T_2^2 - 14T_1T_2 + 9T_1^2 \end{aligned}$$

We disregard the first and solve uniquely for x_2 , recovering x_1 and x_3 in the process.

- (v) Here we find that $x_1 \leq \frac{1}{3}x_2$ and so $\frac{1}{3} \geq \frac{-3(T_1-T_2) \pm (9T_1^2 - 14T_1T_2 + 9T_2^2)^{\frac{1}{2}}}{2T_2}$. Similarly to the two previous cases, we have two inequalities:

$$\begin{aligned} \frac{49}{9}T_2^2 - 14T_1T_2 + 9T_1^2 &< 9T_2^2 - 14T_1T_2 + 9T_1^2 \\ \frac{49}{9}T_2^2 - 14T_1T_2 + 9T_1^2 &> 9T_2^2 - 14T_1T_2 + 9T_1^2 \end{aligned}$$

The second inequality cannot hold and so we disregard it. This allows us to conclude a unique solution (x_1, x_2, x_3) to (4.2).

Note that in cases (iii), (iv) and (v), all $T_i \neq 0$ for $i = 1, 2, 3$. Thus, we may apply lemma 3.2 to conclude that the solution is unique. \square

4.3. The Heisenberg Group, \mathbf{H}_3 .

Theorem 4.3. Let T be a left-invariant $(0, 2)$ -tensor field on \mathbf{H}_3 . There exists a unique left-invariant Riemannian metric g such that $X(g) = T$ if and only if T is diagonalisable in a basis $\{V_i\}_{i=1}^3$ satisfying (1.4) with $\lambda_1 = 2, \lambda_2 = \lambda_3 = 0$ and $T_1 > 0, T_2, T_3 < 0$.

Proof. Fix a basis $\{V_i\}_{i=1}^3$ of the Lie algebra \mathfrak{g} in which T is diagonal and (1.4) holds. We compute the variables $\mathbf{x}_1 = -x_1, \mathbf{x}_2 = x_1, \mathbf{x}_3 = x_1$. This simplifies (2.3) to

$$\begin{cases} T_1 = \frac{x_1^3}{x_2^2 x_3^2} \\ T_2 = \frac{-3x_1^2}{x_2 x_3^2} \\ T_3 = \frac{-3x_1^2}{x_2^2 x_3} \end{cases} \quad (4.3)$$

The second equation becomes $x_2 = \frac{-3x_1^2}{x_3^2 T_2}$. Substituting this into the first gives, $x_1 = \frac{x_3^2 T_2^2}{9T_1}$.

Finally we substitute both expressions into the third equation to find $x_3 = \frac{-27T_1^2}{T_2^2 T_3}$. We compute $x_1 = \frac{81T_1^2}{T_2^2 T_3^2}$ and $x_2 = \frac{-27T_1^2}{T_2 T_3^2}$. As these three expressions depend only on T , there must exist a single metric g solving $X(g) = T$ in our fixed basis. By lemma 3.1, this proves the existence portion of the theorem. Since all $T_i \neq 0$ for $i = 1, 2, 3$, as per § 3, we may apply lemma 3.2 giving us uniqueness of g solving (1.2). \square

4.4. Euclidean Space, \mathbb{R}^3 . Euclidean Space is Ricci-flat and so it has Einstein tensor 0. Thus \mathcal{E} , and subsequently the cross curvature, is not well defined.

REFERENCES

- [Bes87] A. L. Besse, *Einstein manifolds*, Ergebnisse der Mathematik und ihrer Grenzgebiete (3), vol. 10, Springer-Verlag, Berlin, 1987. MR0867684
- [BIS20] Paul Bryan, Mohammad Ivaki, and Julian Scheuer, *Negatively Curved Three-Manifolds, Hyperbolic Metrics, Isometric Embeddings in Minkowski Space and the Cross Curvature Flow*, Handbook of Differential Geometry, 2020, pp. 75–97.
- [BP21] Timothy Buttsworth and Artem Pulemotov, *The prescribed cross curvature problem on the three-sphere*, arXiv preprint (2021), available at [2107.13246](#).
- [But19] Timothy Buttsworth, *The prescribed Ricci curvature problem on three-dimensional unimodular Lie groups*, Math. Nachr. **292** (2019), no. 4, 747–759.
- [CH04] Bennett Chow and Richard S. Hamilton, *The cross curvature flow of 3-manifolds with negative sectional curvature*, Turkish J. Math. **28** (2004), 1–10.
- [dC92] Manfredo P. do Carmo, *Riemannian geometry*, Birkhäuser, 1992.
- [DeT16] Dennis M. DeT16, *Existence of metrics with prescribed Ricci curvature*, Surveys in Differential Geometry, 2016, pp. 525–538.
- [Gki08] Ioannis Gkigkitzis, *On the cross curvature tensor and the cross curvature flow*, PhD Thesis, Columbia University, 2008.
- [Hal15] Brian C. Hall, *Lie groups, Lie algebras, and representations: an elementary introduction*, Springer, 2015.
- [Ham84] Richard S. Hamilton, *The Ricci curvature equation*, Seminar on nonlinear partial differential equations (New York, NY, 1983), Springer New York, 1984, pp. 47–72.
- [HL09] Ku Yong Ha and Jong Bum Lee, *Left invariant metrics and curvatures on simply connected three-dimensional Lie groups*, Math. Nachr. **282** (2009), no. 6, 868–898.
- [Lee18] John M. Lee, *Introduction to Riemannian manifolds*, 2nd ed., Graduate Texts in Mathematics, vol. 176, Springer, Cham, 2018.